randhash proof (2 admits)

proof/correctness/Correctness_Hash.ec
@@ -113,49 +113,18 @@ seq 1 0 : (
     + auto => /> *; rewrite !/to_list !/mkseq -!iotaredE => /> /#. 
 qed.
 
-require import Types.
-
-op H (pad a b : nbytes) : nbytes = Hash (pad ++ a ++ b).
-op rand_hash_padding : W64.t = W64.one.
-
-module RandHash = {
-proc rand_hash (_left _right : nbytes, _seed : nbytes, address : adrs) : nbytes * adrs = { 
-  var padding : W8.t list;
-  var key : W8.t list;
-  var bitmask_0, bitmask_1 : nbytes;
-  var buf : W8.t list;
-  var addr_bytes : W8.t list;
-
-  padding <@ Util.w64_to_bytes (rand_hash_padding, padding_len);
-
-  address <- set_key_and_mask address 0;
-  addr_bytes <- addr_to_bytes address;
-  key <@ Hash.prf (addr_bytes, _seed);
-
-  address <- set_key_and_mask address 1;
-  addr_bytes <- addr_to_bytes address;
-  bitmask_0 <@ Hash.prf (addr_bytes,  _seed);
-
-  address <- set_key_and_mask address 2;
-  addr_bytes <- addr_to_bytes address;
-  bitmask_1 <@ Hash.prf (addr_bytes,  _seed);
-
-  buf <- (nbytexor _left bitmask_0) ++ (nbytexor _right bitmask_1);
-  
-  return (H padding key buf, address);
-  }
-}.
-
-
 op merge_nbytes_to_array (a b : nbytes) : W8.t Array64.t = 
   Array64.init (fun i => if 0 <= i < 32 then nth witness a i else nth witness b (i - 32)).
 
 lemma rand_hash_correct (i0 i1: nbytes, _pub_seed : W8.t Array32.t, _in : W8.t Array64.t, a : W32.t Array8.t) :
     padding_len = XMSS_PADDING_LEN /\ 
     prf_padding_val = XMSS_HASH_PADDING_PRF /\
-    padding_len = XMSS_PADDING_LEN =>
+    padding_len = XMSS_PADDING_LEN /\ 
+    n = XMSS_N /\
+    size i0 = n /\ 
+    size i1 = n =>
     equiv [
-      M(Syscall).__thash_h ~ RandHash.rand_hash :
+      M(Syscall).__thash_h ~ Hash.rand_hash :
       arg{1}.`2 = (merge_nbytes_to_array i0 i1) /\
       arg{1}.`3 = _pub_seed /\
       arg{1}.`4 = a /\
@@ -165,24 +134,27 @@ lemma rand_hash_correct (i0 i1: nbytes, _pub_seed : W8.t Array32.t, _in : W8.t A
       res{1}.`2 = res{2}.`2
     ].
 proof.
-move => *.
+move => [#] *.
 proc; auto => />.
 conseq (: 
   (forall (k : int), 0 <= k < 32 => in_0{1}.[k] = nth witness _left{2} k) /\
   (forall (k : int), 0 <= k < 32 => in_0{1}.[32 + k] = nth witness _right{2} k) /\
   _seed{2} = to_list pub_seed{1} /\ 
-  address{2} = addr{1}
-  ==> _
+  address{2} = addr{1} /\
+  size _left{2} = n /\
+  size _right{2} = n
+  ==> 
 ); first by auto => />; rewrite /merge_nbytes_to_array; smt(@List @Array64).
 seq 3 0 : (#pre); 1:auto.
-seq 1 1 : (#pre /\ padding{2} = to_list aux{1}); first by call {1} (ull_to_bytes_correct W64.one); auto => /> /#.  
-swap {1} [2..3] -1. 
+seq 1 1 : (#pre /\ padding{2} = to_list aux{1}); first by call {1} (ull_to_bytes_correct W64.one); auto => /> /#.
+swap {1} [2..3] -1.
 seq 2 2 : (#pre /\ addr_bytes{2} = to_list addr_as_bytes{1}).
-    + inline {1} M(Syscall).__set_key_and_mask; ecall {1} (addr_to_bytes_correctness addr{1}); auto => /> /#.
+    + inline {1} M(Syscall).__set_key_and_mask; ecall {1} (addr_to_bytes_correctness addr{1}); auto => /> /#. 
 seq 1 0 : (
   #pre /\
   forall (k : int), 0 <= k < 32 => buf{1}.[k] = nth witness padding{2} k
 ); first by auto => /> *; smt(@Array128).
+
 seq 1 1 : (
   (forall (k : int), 0 <= k < 32 => in_0{1}.[k] = nth witness _left{2} k) /\
   (forall (k : int), 0 <= k < 32 => in_0{1}.[32 + k] = nth witness _right{2} k) /\
@@ -190,18 +162,22 @@ seq 1 1 : (
   address{2} = addr{1} /\
   addr_bytes{2} = to_list addr_as_bytes{1} /\
   key{2} = to_list aux{1} /\
+  size _left{2} = n /\
+  size _right{2} = n /\
 
   (* Towards #post *)
   forall (k : int), 0 <= k < 32 => buf{1}.[k] = nth witness padding{2} k
 ).
     + inline {1} M(Syscall).__prf_ M(Syscall)._prf; wp; sp.
-      exists * in_01{1}, key0{1}; elim * => _P1 _P2; call {1} (prf_correctness _P1 _P2); [ smt() | auto => /> ]. 
+      exists * in_01{1}, key0{1}; elim * => _P1 _P2; call {1} (prf_correctness _P1 _P2); auto => />. 
 seq 1 0 : (
     #pre /\
     forall (k : int), 0 <= k < 32 => buf{1}.[32 + k] = nth witness key{2} k
 ); first by auto => />; smt(@Array128).
+
 seq 2 2 : (#pre).
     + inline {1} M(Syscall).__set_key_and_mask; ecall {1} (addr_to_bytes_correctness addr{1}); auto => /> /#.
+
 seq 2 1 : (
   (forall (k : int), 0 <= k < 32 => in_0{1}.[k] = nth witness _left{2} k) /\
   (forall (k : int), 0 <= k < 32 => in_0{1}.[32 + k] = nth witness _right{2} k) /\
@@ -211,43 +187,38 @@ seq 2 1 : (
   
   (* Bitmask *)
   (forall (k : int), 0 <= k < 32 => bitmask{1}.[k] = nth witness bitmask_0{2} k) /\
+  size bitmask_0{2} = n /\
 
   (* Towards #post *)
   (forall (k : int), 0 <= k < 32 => buf{1}.[k] = nth witness padding{2} k) /\
   (forall (k : int), 0 <= k < 32 => buf{1}.[32 + k] = nth witness key{2} k)
 ).
     + inline {1} M(Syscall).__prf_ M(Syscall)._prf; wp; sp.
-      exists * in_01{1}, key0{1}; elim * => _P1 _P2; call {1} (prf_correctness _P1 _P2); [ smt() | auto => /> *; smt(@Array64) ].
+      exists * in_01{1}, key0{1}; elim * => _P1 _P2; call {1} (prf_correctness _P1 _P2); auto => /> *; split; [ smt(@Array64) | rewrite size_to_list /# ].
 seq 2 2 : (#pre).
     + inline {1} M(Syscall).__set_key_and_mask; ecall {1} (addr_to_bytes_correctness addr{1}); auto => /> /#.
 seq 2 1 : (
   #pre /\ 
-  (forall (k : int), 0 <= k < 32 => bitmask{1}.[32 + k] = nth witness bitmask_1{2} k)
+  (forall (k : int), 0 <= k < 32 => bitmask{1}.[32 + k] = nth witness bitmask_1{2} k) /\
+  size bitmask_1{2} = n
 ).
     + inline {1} M(Syscall).__prf_ M(Syscall)._prf; wp; sp.
-      exists * in_01{1}, key0{1}; elim * => _P1 _P2; call {1} (prf_correctness _P1 _P2); [ smt() | auto => /> *; smt(@Array64) ].
+      exists * in_01{1}, key0{1}; elim * => _P1 _P2; call {1} (prf_correctness _P1 _P2); auto => /> *; do split;1,2:smt(@Array64); rewrite size_to_list /#.
 
-(* WIP: Maybe use a conseq here to simplify #post *)
 
-(* 
-seq 2 0 : (
-  #pre /\
-  to_list buf{1} = padding{2} ++ nbytexor _left{2} bitmask_0{2} ++ nbytexor _right{2} bitmask_1{2}
-).
-    + admit.
-inline {1} M(Syscall)._core_hash_128; wp; sp.
-ecall {1} (hash_128 in_00{1}).
-skip => /> &1 &2 *.
-rewrite /nbytexor /H.
-rewrite /to_list /mkseq -!iotaredE => />.
+inline {1}  M(Syscall)._core_hash_128. wp. ecall {1} (hash_128 in_00{1}).
+auto => />. (* Simplifies #post *)
 
-(* while starts here *)
-
-while (
-  0 <= i{1} <= 64 /\
-  
-)
-*)
-
-admit.
+while {1} (
+  0 <= to_uint i{1} <= 64 /\
+  addr{1} = address{2} /\ 
+  (forall (k : int), 0 <= k < 32 => buf{1}.[k] = nth witness padding{2} k) /\
+  (forall (k : int), 0 <= k < 32 => buf{1}.[32 + k] = nth witness key{2} k) /\
+  (forall (k : int), 0 <= k < to_uint i{1} => buf{1}.[64 + to_uint i{1}] = nth witness ((Primitives.nbytexor _left{2} bitmask_0{2}) ++ (Primitives.nbytexor _right{2} bitmask_1{2})  ) (to_uint i{1}) )
+) (64 - to_uint i{1}).
+    + auto => /> &hr *. do split;1,2,6:smt(@W64 pow2_64).
+        * move => ???; rewrite get_setE; [ smt(@W64 pow2_64) | smt(@Array64 @List @W64 pow2_64) ].
+        * move => ???; rewrite get_setE; [ smt(@W64 pow2_64) | smt(@Array64 @List @W64 pow2_64) ].
+        * move => ???; rewrite get_setE; first by smt(@W64 pow2_64). rewrite ifF; first by smt(@W64 pow2_64). admit.
+    + auto => /> &1 &2 *. split; 1:smt(). move => *. split; 1:smt(@W64 pow2_64). move => ??????? H. rewrite H. congr. admit. (* smt(@List @Array128). *)
 qed.
